finish key lemma showing preservation of unprocessed stack symbols invariant

coq/Parser_complete.v
@@ -2,8 +2,9 @@ Require Import List String.
 Require Import GallStar.Defs.
 Require Import GallStar.Lex.
 Require Import Prediction.
-(*Require Import GallStar.Parser.*)
 Require Import GallStar.Prediction_error_free.
+Require Import GallStar.Prediction_complete.
+Require Import GallStar.Parser.
 Require Import GallStar.Parser_error_free.
 Require Import GallStar.Tactics.
 Require Import GallStar.Utils.
@@ -12,6 +13,40 @@ Import ListNotations.
 
 (* a thought: maybe replace this invariant with a function of
    the stack, i.e., "unprocessed symbols" *)
+
+(*
+Inductive unproc_tail_syms_recognize (g : grammar) : list frame -> list token -> Prop :=
+| TR_nil :
+    unproc_tail_syms_recognize g [] []
+| TR_cons :
+    forall o pre x suf v w w' frs,
+      gamma_recognize g suf w
+      -> unproc_tail_syms_recognize g frs w'
+      -> unproc_tail_syms_recognize g (Fr (Loc o pre (NT x :: suf)) v :: frs) (w ++ w').
+
+Hint Constructors unproc_tail_syms_recognize.
+
+Inductive unproc_stack_syms_recognize (g : grammar) : parser_stack -> list token -> Prop :=
+| SR :
+    forall o pre suf v w w' frs,
+      gamma_recognize g suf w
+      -> unproc_tail_syms_recognize g frs w'
+      -> unproc_stack_syms_recognize g (Fr (Loc o pre suf) v, frs) (w ++ w').
+
+Hint Constructors unproc_stack_syms_recognize.
+
+
+Lemma ussr_inv :
+  forall g o pre suf v frs w'',
+    unproc_stack_syms_recognize g (Fr (Loc o pre suf) v, frs) w''
+    -> exists w w',
+      w'' = w ++ w'
+      /\ gamma_recognize g suf w
+      /\ unproc_tail_syms_recognize g frs w'.
+Proof.
+  intros g o pre suf v frs w'' hs; inv hs; eauto.
+Qed.
+*)
 
 Inductive unproc_tail_syms_recognize (g : grammar) : list frame -> list token -> Prop :=
 | TR_nil :
@@ -44,6 +79,124 @@ Proof.
   intros g o pre suf v frs w'' hs; inv hs; eauto.
 Qed.
 
+Fixpoint unprocStackSyms' (stk : parser_stack) : list symbol :=
+  unprocStackSyms (lstackOf stk).
+
+Lemma return_preserves_ussr :
+  forall g ce cr cr' frs x o o' pre pre' suf' v v' w,
+    ce = Fr (Loc o pre []) v
+    -> cr  = Fr (Loc o' pre' (NT x :: suf')) v'
+    -> cr' = Fr (Loc o' (pre' ++ [NT x]) suf') (v' ++ [Node x v])
+    -> gamma_recognize g (unprocStackSyms' (ce, cr :: frs)) w
+    -> gamma_recognize g (unprocStackSyms' (cr', frs)) w.
+Proof.
+  intros g ce cr cr' frs x o o' pre pre' suf' v v' w
+         ? ? ? hs; subst; auto.
+Qed.
+
+Lemma consume_preserves_ussr :
+  forall g fr fr' frs o pre suf a l v w,
+    fr = Fr (Loc o pre (T a :: suf)) v
+    -> fr' = Fr (Loc o (pre ++ [T a]) suf) (v ++ [Leaf l])
+    -> gamma_recognize g (unprocStackSyms' (fr, frs)) ((a, l) :: w)
+    -> gamma_recognize g (unprocStackSyms' (fr', frs)) w.
+Proof.
+  intros g fr fr' frs o pre suf a l v w ? ? hs; subst; sis.
+  apply gamma_recognize_terminal_head in hs.
+  destruct hs as [l' [w' [heq hg]]]. 
+  inv heq; auto.
+Qed.
+
+Lemma push_succ_preserves_ussr :
+  forall g fr o pre x suf v frs w rhs,
+    fr = Fr (Loc o pre (NT x :: suf)) v
+    -> no_left_recursion g
+    -> stack_wf g (fr, frs)
+    -> llPredict g x (lstackOf (fr, frs)) w = PredSucc rhs
+    -> gamma_recognize g (unprocStackSyms' (fr, frs)) w
+    -> gamma_recognize g (unprocStackSyms' (Fr (Loc (Some x) [] rhs) [], fr :: frs)) w.
+Proof.
+  intros g fr o pre x suf v frs w rhs heq hn hw hl hu; subst; sis.
+  apply gamma_recognize_nonterminal_head in hu.
+  destruct hu as [rhs' [wpre [wmidsuf [heq [hin [hg hg']]]]]]; subst.
+  apply gamma_recognize_split in hg'.
+  destruct hg' as [wmid [wsuf [? [hg' hg'']]]]; subst.
+  eapply llPredict_succ_at_most_one_rhs_applies in hl; eauto; sis; subst;
+  (do 2 (apply gamma_recognize_app; auto)).
+Qed.
+
+Lemma push_ambig_preserves_ussr :
+  forall g fr o pre x suf v frs w rhs,
+    fr = Fr (Loc o pre (NT x :: suf)) v
+    -> no_left_recursion g
+    -> stack_wf g (fr, frs)
+    -> llPredict g x (lstackOf (fr, frs)) w = PredAmbig rhs
+    -> gamma_recognize g (unprocStackSyms' (fr, frs)) w
+    -> gamma_recognize g (unprocStackSyms' (Fr (Loc (Some x) [] rhs) [], fr :: frs)) w.
+Proof.
+  intros g fr o pre x suf v frs w rhs ? hn hw hl hu; subst; sis.
+  eapply llPredict_ambig_rhs_unproc_stack_syms in hl; eauto.
+  sis; auto.
+Qed.
+
+Lemma step_preserves_ussr :
+  forall g av av' stk stk' w w' u u',
+    no_left_recursion g
+    -> stack_wf g stk
+    -> gamma_recognize g (unprocStackSyms' stk) w
+    -> step g (Pst av stk w u) = StepK (Pst av' stk' w' u')
+    -> gamma_recognize g (unprocStackSyms' stk') w'.
+Proof.
+  intros g av av' stk stk' w w' u u' hn hw hu hs.
+  unfold step in hs; dmeqs h; tc; inv hs.
+  - eapply return_preserves_ussr; eauto.
+  - eapply consume_preserves_ussr; eauto.
+  - eapply push_succ_preserves_ussr; eauto.
+  - eapply push_ambig_preserves_ussr; eauto.
+Qed.
+
+Lemma ussr_implies_multistep_doesn't_reject :
+  forall (g : grammar) 
+         (tri : nat * nat * nat)
+         (a   : Acc lex_nat_triple tri)
+         (av  : NtSet.t)
+         (stk : parser_stack)
+         (w   : list token)
+         (u   : bool)
+         (a   : Acc lex_nat_triple (meas g (Pst av stk w u)))
+         (s   : string),
+    tri = meas g (Pst av stk w u)
+    -> no_left_recursion g
+    -> stack_wf g stk
+    -> gamma_recognize g (unprocStackSyms' stk) w
+    -> multistep g (Pst av stk w u) a <> Reject s.
+Proof.
+  intros g tri a.
+  induction a as [tri hlt IH].
+  intros av stk w u a s heq hn hw hu; unfold not; intros hm; subst.
+  apply multistep_reject_cases in hm.
+  destruct hm as [hs | [st' [a' [hs hm]]]]. 
+  - (* lemma *)
+    clear a hlt IH.
+    unfold step in hs; dmeqs h; tc; inv hs; sis; inv hu.
+    + inv H2. 
+      inv H1.
+    + inv H2.
+      inv H1.
+      tc.
+    + admit.
+    + inv H1.
+      apply lhs_mem_allNts_true in H0. tc.
+  - destruct st' as [av' stk' w' u']. 
+    eapply IH with (y := meas g (Pst av' stk' w' u')); eauto.
+    + apply step_meas_lt; auto.
+    + eapply step_preserves_stack_wf_invar; eauto. 
+    + eapply step_preserves_ussr; eauto.
+Admitted.
+Print Assumptions ussr_implies_multistep_doesn't_reject.
+
+
+
 Lemma return_preserves_ussr :
   forall g ce cr cr' frs x o o' pre pre' suf' v v' w,
     ce = Fr (Loc o pre []) v
@@ -73,6 +226,74 @@ Proof.
   destruct hg as [l' [w' [? hg]]]; subst.
   inv heq; auto.
 Qed.
+
+(* replace this with something better *)
+Lemma unproc_tail_syms_unprocTailSyms :
+  forall g frs w,
+    unproc_tail_syms_recognize g frs w
+    -> gamma_recognize g (unprocTailSyms (map loc frs)) w.
+Proof.
+  intros g frs; induction frs as [| fr frs IH]; intros w hu; sis; inv hu; auto.
+  sis. apply gamma_recognize_app; auto.
+Qed.
+
+Lemma push_succ_preserves_ussr :
+  forall g fr o pre x suf v frs w rhs,
+    fr = Fr (Loc o pre (NT x :: suf)) v
+    -> no_left_recursion g
+    -> stack_wf g (fr, frs)
+    -> llPredict g x (lstackOf (fr, frs)) w = PredSucc rhs
+    -> unproc_stack_syms_recognize g (fr, frs) w
+    -> unproc_stack_syms_recognize g (Fr (Loc (Some x) [] rhs) [], fr :: frs) w.
+Proof.
+  intros g fr o pre x suf v frs w rhs heq hn hw hl hu; subst; sis.
+  eapply ussr_inv in hu.
+  destruct hu as [wpremid [wsuf [heq [hg ht]]]]; subst.
+  apply gamma_recognize_nonterminal_head in hg.
+  destruct hg as [rhs' [wpre [wmid [heq [hin [hg hg']]]]]]; subst.
+  rewrite <- app_assoc; constructor; auto.
+  eapply llPredict_succ_at_most_one_rhs_applies in hl; eauto.
+  - subst; auto.
+  - sis.
+    rewrite <- app_assoc.
+    do 2 (apply gamma_recognize_app; auto).
+    apply unproc_tail_syms_unprocTailSyms; auto.
+Qed.
+
+Lemma push_ambig_preserves_ussr :
+  forall g fr o pre x suf v frs w rhs,
+    fr = Fr (Loc o pre (NT x :: suf)) v
+    -> no_left_recursion g
+    -> stack_wf g (fr, frs)
+    -> llPredict g x (lstackOf (fr, frs)) w = PredAmbig rhs
+    -> unproc_stack_syms_recognize g (fr, frs) w
+    -> unproc_stack_syms_recognize g (Fr (Loc (Some x) [] rhs) [], fr :: frs) w.
+Proof.
+  intros g fr o pre x suf v frs w rhs ? hn hw hl hu; subst; sis.
+  eapply ussr_inv in hu.
+  destruct hu as [wpremid [wsuf [heq [hg ht]]]]; subst.
+  apply gamma_recognize_nonterminal_head in hg.
+  destruct hg as [rhs' [wpre [wmid [heq [hin [hg hg']]]]]]; subst.
+  eapply llPredict_ambig_rhs_unproc_stack_syms in hl; eauto; sis.
+  rewrite <- app_assoc in *.
+  constructor.
+  
+
+Lemma step_preserves_ussr :
+  forall g av av' stk stk' w w' u u',
+    no_left_recursion g
+    -> stack_wf g stk
+    -> unproc_stack_syms_recognize g stk w
+    -> step g (Pst av stk w u) = StepK (Pst av' stk' w' u')
+    -> unproc_stack_syms_recognize g stk' w'.
+Proof.
+  intros g av av' stk stk' w w' u u' hn hw hu hs.
+  unfold step in hs; dmeqs h; tc; inv hs; sis.
+  - eapply return_preserves_ussr; eauto.
+  - eapply consume_preserves_ussr; eauto.
+  - eapply push_succ_preserves_ussr; eauto.
+  - admit.
+Admitted.
 
 Fixpoint processedSyms' (frs : list location) : list symbol :=
   match frs with 
